Clap/eDSLState/HashCons/HashConsM.lean
@@ -21,7 +21,7 @@ def saveExpr (e : CacheExpr p) : HashConsM p ExprRef := do
   else if h : e.wellFormed state.size then
     let post_state := state.pushExpr e h
     set post_state
-    return state.exprs.size
+    return state.size
   else pure 42
 
 variable {e : CacheExpr p} {σ : HashConsSt p}
@@ -45,14 +45,34 @@ def wellFormed
 : Prop :=
   σ.exprs.isPrefixOf (action.getHashConsState σ).exprs
 
-@[grind .]
-lemma run_saveExpr_of_wellFormed (h : e.wellFormed σ.exprs.size) :
+@[grind =]
+lemma run_saveExpr_of_wellFormed (h : e.wellFormed σ.size) :
   (HashConsM.saveExpr e).run σ =
   if e ∈ σ.exprs
   then (σ.exprs.idxOf e, σ)
-  else (σ.exprs.size, HashConsSt.pushExpr e σ h)
+  else (σ.size, HashConsSt.pushExpr e σ h)
 := by
   unfold HashConsM.saveExpr run
+  grind
+
+@[grind =]
+lemma getResult_saveExpr_of_wellFormed (h : e.wellFormed σ.size) :
+  (HashConsM.saveExpr e).getResult σ =
+  if e ∈ σ.exprs
+  then σ.exprs.idxOf e
+  else σ.size
+:= by
+  unfold getResult
+  grind
+
+@[grind =]
+lemma getHashConsState_saveExpr_of_wellFormed (h : e.wellFormed σ.size) :
+  (HashConsM.saveExpr e).getHashConsState σ =
+  if e ∈ σ.exprs
+  then σ
+  else HashConsSt.pushExpr e σ h
+:= by
+  unfold getHashConsState
   grind
 
 lemma run_saveExpr_of_mem (h : e ∈ σ) :
@@ -71,7 +91,7 @@ end SaveExpr
 section Membership
 
 instance : Membership ExprRef (HashConsSt p) where
-  mem coll ref := ref < coll.exprs.size
+  mem coll ref := ref < coll.size
 
 variable {σ : HashConsSt p} {ref : ExprRef}
 
@@ -137,7 +157,7 @@ lemma run_mkVar :
   (mkVar e!).run σ =
   if (.v e!) ∈ σ.exprs
   then (σ.exprs.idxOf (.v e!), σ)
-  else (σ.exprs.size, σ.pushExpr (.v e!) (by simp)) :=
+  else (σ.size, σ.pushExpr (.v e!) (by simp)) :=
   run_saveExpr_of_wellFormed wellFormed_v
 
 @[simp, grind =]
@@ -198,6 +218,174 @@ lemma wellFormed_mkSub {l r} : (mkSub l r).wellFormed σ := by
 
 @[simp, grind .]
 lemma wellFormed_mkMul {l r} : (mkMul l r).wellFormed σ := by
+  unfold mkMul
+  grind
+
+@[grind .]
+lemma getResult_mkConstant {c}
+:
+  (mkConstant c).getResult σ =
+  if (.c c) ∈ σ.exprs
+  then σ.exprs.idxOf (.c c)
+  else σ.size
+:= by
+  unfold getResult mkConstant
+  grind
+
+@[grind .]
+lemma getHashConsState_mkConstant {c}
+:
+  (mkConstant c).getHashConsState σ =
+  if (.c c) ∈ σ.exprs
+  then σ
+  else σ.pushExpr (.c c) (by grind)
+:= by
+  unfold getHashConsState mkConstant
+  grind
+
+@[grind .]
+lemma getResult_lt_getHashConsState_size_mkConstant {c}
+:
+  (mkConstant c).getResult σ < ((mkConstant c).getHashConsState σ).size
+:= by
+  unfold mkConstant
+  grind
+
+@[grind .]
+lemma getResult_mkVar {c}
+:
+  (mkConstant c).getResult σ =
+  if (.c c) ∈ σ.exprs
+  then σ.exprs.idxOf (.c c)
+  else σ.size
+:= by
+  unfold getResult mkConstant
+  grind
+
+@[grind .]
+lemma getHashConsState_mkVar {v}
+:
+  (mkVar v).getHashConsState σ =
+  if (.v v) ∈ σ.exprs
+  then σ
+  else σ.pushExpr (.v v) (by grind)
+:= by
+  unfold getHashConsState mkVar
+  grind
+
+@[grind .]
+lemma getResult_lt_getHashConsState_size_mkVar {v}
+:
+  (mkVar v).getResult σ < ((mkVar v).getHashConsState σ).size
+:= by
+  unfold mkVar
+  grind
+
+@[grind .]
+lemma getResult_mkAdd_of_wellFormed {l r}
+  (h_l : l < σ.size)
+  (h_r : r < σ.size)
+:
+  (mkAdd l r).getResult σ =
+  if (.binary_op l r .add) ∈ σ.exprs
+  then σ.exprs.idxOf (.binary_op l r .add)
+  else σ.size
+:= by
+  unfold getResult mkAdd
+  grind
+
+@[grind .]
+lemma getHashConsState_mkAdd_of_wellFormed {l r}
+  (h_l : l < σ.size)
+  (h_r : r < σ.size)
+:
+  (mkAdd l r).getHashConsState σ =
+  if (.binary_op l r .add) ∈ σ.exprs
+  then σ
+  else HashConsSt.pushExpr (.binary_op l r .add) σ (by grind)
+:= by
+  unfold mkAdd
+  grind
+
+@[grind .]
+lemma getResult_lt_getHashConsState_size_mkAdd {l r}
+  (h_l : l < σ.size)
+  (h_r : r < σ.size)
+:
+  (mkAdd l r).getResult σ < ((mkAdd l r).getHashConsState σ).size
+:= by
+  unfold mkAdd
+  grind
+
+@[grind .]
+lemma getResult_mkSub_of_wellFormed {l r}
+  (h_l : l < σ.size)
+  (h_r : r < σ.size)
+:
+  (mkSub l r).getResult σ =
+  if (.binary_op l r .sub) ∈ σ.exprs
+  then σ.exprs.idxOf (.binary_op l r .sub)
+  else σ.size
+:= by
+  unfold getResult mkSub
+  grind
+
+@[grind .]
+lemma getHashConsState_mkSub_of_wellFormed {l r}
+  (h_l : l < σ.size)
+  (h_r : r < σ.size)
+:
+  (mkSub l r).getHashConsState σ =
+  if (.binary_op l r .sub) ∈ σ.exprs
+  then σ
+  else HashConsSt.pushExpr (.binary_op l r .sub) σ (by grind)
+:= by
+  unfold mkSub
+  grind
+
+@[grind .]
+lemma getResult_lt_getHashConsState_size_mkSub {l r}
+  (h_l : l < σ.size)
+  (h_r : r < σ.size)
+:
+  (mkSub l r).getResult σ < ((mkSub l r).getHashConsState σ).size
+:= by
+  unfold mkSub
+  grind
+
+@[grind .]
+lemma getResult_mkMul_of_wellFormed {l r}
+  (h_l : l < σ.size)
+  (h_r : r < σ.size)
+:
+  (mkMul l r).getResult σ =
+  if (.binary_op l r .mul) ∈ σ.exprs
+  then σ.exprs.idxOf (.binary_op l r .mul)
+  else σ.size
+:= by
+  unfold getResult mkMul
+  grind
+
+@[grind .]
+lemma getHashConsState_mkMul_of_wellFormed {l r}
+  (h_l : l < σ.size)
+  (h_r : r < σ.size)
+:
+  (mkMul l r).getHashConsState σ =
+  if (.binary_op l r .mul) ∈ σ.exprs
+  then σ
+  else HashConsSt.pushExpr (.binary_op l r .mul) σ (by grind)
+:= by
+  unfold mkMul
+  grind
+
+@[grind .]
+lemma getResult_lt_getHashConsState_size_mkMul {l r}
+  (h_l : l < σ.size)
+  (h_r : r < σ.size)
+:
+  (mkMul l r).getResult σ < ((mkMul l r).getHashConsState σ).size
+:= by
   unfold mkMul
   grind
 
